AutomataTheory/Congruences/Basic.lean
@@ -5,6 +5,7 @@ Authors: Ching-Tsun Chou
 -/
 
 import AutomataTheory.Sequences.Basic
+import AutomataTheory.Languages.Basic
 
 /-!
 A congruence is an equivalence relation on finite sequences that is
@@ -13,10 +14,53 @@ For now, we assume only the right congruence condition.  We will
 add the left congruence condition if and when it is needed.
 -/
 
+open Function Set
+
 section Congruences
+
+open Classical
 
 class Congruence (A : Type*) extends eq : Setoid (List A) where
 --  left_congr : ∀ u v, eq u v → ∀ w, eq (w ++ u) (w ++ v)
   right_congr : ∀ u v, eq u v → ∀ w, eq (u ++ w) (v ++ w)
+
+variable {A : Type*}
+
+def Congruence.QuotType (c : Congruence A) := Quotient c.eq
+
+def Congruence.EqvCls (c : Congruence A) (s : c.QuotType) : Set (List A) :=
+  (Quotient.mk c.eq) ⁻¹' {s}
+
+def Congruence.ConcatOmegaLang (c : Congruence A) (s t : c.QuotType) : Set (ℕ → A) :=
+  ConcatOmega (c.EqvCls s) (c.EqvCls t)
+
+def Congruence.Saturates (c : Congruence A) (L : Set (ℕ → A)) :=
+  ∀ s t : c.QuotType, (c.ConcatOmegaLang s t ∩ L).Nonempty → c.ConcatOmegaLang s t ⊆ L
+
+def Congruence.Ample (c : Congruence A) :=
+  ∀ as, ∃ s t : c.QuotType, as ∈ c.ConcatOmegaLang s t
+
+variable {c : Congruence A}
+
+theorem congruence_saturates_compl {L : Set (ℕ → A)}
+    (h_sat : c.Saturates L) : c.Saturates Lᶜ := by
+  rintro s t ⟨as, h_as, h_as_c⟩ as' h_as'
+  by_contra h_contra
+  simp at h_contra
+  have h_l : (c.ConcatOmegaLang s t ∩ L).Nonempty := by
+    use as' ; simp [h_as', h_contra]
+  have := h_sat s t h_l h_as
+  contradiction
+
+theorem congruence_ample_saturates_union {L : Set (ℕ → A)}
+    (h_amp : c.Ample) (h_sat : c.Saturates L) :
+    L =  ⋃ s, ⋃ t, if (c.ConcatOmegaLang s t ∩ L).Nonempty then c.ConcatOmegaLang s t else ∅ := by
+  ext as ; simp ; constructor
+  · intro h_l
+    obtain ⟨s, t, h_st⟩ := h_amp as
+    use s, t ; simp [h_st]
+    use as ; simp [h_st, h_l]
+  · rintro ⟨s, t, h_ne, h_as⟩
+    exact h_sat s t h_ne h_as
 
 end Congruences
